```math
Y ^{S} = Y ^{D}
```

```math
Y ^{D}_{0}
=
D _{0} \left(
    \dfrac{E _{0} \cdot P ^{*}}{
        P
    },
    Y - \overline{T},
    \overline{I},
    \overline{G}
\right)
```

```math
Y ^{D} = C + I + G + \left(
    X-M
\right)
```


```math
E _{0}
```

```math
1. \ E _{1} \uparrow \\
\Downarrow \\
Y ^{D}_{1}
=
D _{1} \left(
    \dfrac{E _{1} \cdot P ^{*}}{
        P
    },
    Y - \overline{T},
    \overline{I},
    \overline{G}
\right) \uparrow\\
\Downarrow \\
\left(
    E _{0}, Y _{0}
\right) \Rightarrow 
\left(
    E _{1}, Y _{1}
\right)\\
 \ \\
\therefore  DD곡선\ 우상향


```

```math
\dfrac{ \overline{M ^{S}}}{P} 
```


```math
\dfrac{M ^{D}}{P} = L \left(
    R, Y _{0}
\right)
```


```math
\dfrac{ \overline{M ^{S}}}{P}
= \dfrac{M ^{D}}{P} \\ \Downarrow \\
R _{0}

```

```math
R _{0} = DR
```

```math
FR = R ^{*} + \dfrac{E ^{e}}{E} - 1
```

```math
DR = FR \\
\Downarrow \\
E _{0}

```

```math

```


```math
y _{0}  \Rightarrow y _{1}\uparrow \\ \Downarrow\\
\dfrac{M ^{D}}{P} _{1} \uparrow  = L \left(
    R, Y _{1} \uparrow 
\right)\uparrow \\\Downarrow \\
R _{0} \Rightarrow R _{1} \uparrow \\
\Downarrow \\
E _{0} \Rightarrow E _{1} \Downarrow 
```

```math
E \uparrow \Rightarrow \left(
\begin{array}{c}
 X \uparrow \\ M \downarrow 
\end{array}
\right) \Rightarrow CA \uparrow
``` 

```math
\eta + \eta ^{*} > 1
```
