```math
   \dfrac{M^d}{P}
    = \dfrac{M^s}{P}
    = \dfrac{M}{P}
```
```math
\dfrac{M^d}{P}=\dfrac{M^s}{P}=\dfrac{M}{P}
```
```math
E_{\$ / €} = c \cdot 
\dfrac
{P_{US}}
{P_{EU}}
```
```math
E_{\$/€}=c\cdot\dfrac{P_{US}}{P_{EU}}
```
```math
E_{\text{\$/€}}=c\times\dfrac{\dfrac{M_{US}}{M_{EU}}}{\dfrac{L\left(R_\text{€},Y_{US}\right)}{L\left(R_\text{€},Y_{US}\right)}}
```
```math
\dfrac{
    \dot{P}
}{
    P
}
= \dfrac{
    \dot{M}
}{
    M
}
= \dfrac
{
    \dot{Y}
}{
    Y
}
```
```math
\dfrac{\dot{P}}{P}=\dfrac{\dot{M}}{M}=\dfrac{\dot{Y}}{Y}
```
```math
\pi^{US}_{t}=\mu^{US}_{t}-\text{g}^{US}_t
```

```math
M^d = \bar{\text{L}} \cdot \text{P} \cdot \text{Y} \\\Rightarrow \dfrac{\text{M}}{\text{P}}
= \bar{\text{L}} \cdot \text{Y} \\
\Rightarrow \dfrac{\dot{P}}{P}=\dfrac{\dot{M}}{M}-\dfrac{\dot{\bar{L}}}{\bar{L}}-\dfrac{\dot{Y}}{Y}\\\dfrac{\dot{\bar{L}}}{\bar{L}} = 0 \\
\Rightarrow\pi^{US}_{t}=\mu^{US}_{t}-\text{g}^{US}_t
```

```math
E_{\$/€}=c\cdot\dfrac{P_{US}}{P_{EU}}
\\\Rightarrow
\dfrac{\dot{E}}{E}=
\dfrac{\dot{C}}{C}+
\dfrac{\dot{P}_{US}}{P_{US}}-
\dfrac{\dot{P_{EU}}}{P_{EU}} 
\left( \dfrac{\dot{C}}{C} \right)
\\\Rightarrow
\dfrac{\dot{E}}{E}=
\pi^{US}_t-
\pi^{EU}_t
```

```math
\dfrac{\dot{E}}{E}=\pi^{US}_t-\pi^{EU}_t
\\ = 
\left( 
    \mu^{US}_{t}-\text{g}^{US}_t    
\right)
-
\left( 
    \mu^{EU}_{t}-\text{g}^{EU}_t
\right)
\\=
\left( 
    \mu^{US}_{t}-\mu^{EU}_{t}
\right)
-
\left( 
   \text{g}^{US}_t -\text{g}^{EU}_t
\right)\\

\therefore\dfrac{\dot{E}}{E}
=\left( 
    \mu^{US}_{t}-\mu^{EU}_{t}
\right)
-
\left( 
   \text{g}^{US}_t -\text{g}^{EU}_t
\right)\\
```